work on lifting.v for islaris

islaris/opsem_itree.v
@@ -1,7 +1,18 @@
 From ITree Require Import ITree Recursion RecursionFacts InterpFacts Eqit.
-From iris.itree Require Import wpi choice ub state handler itree halt.
+From iris.itree Require Import wpi choice ub state handler itree halt later.
 Require Export isla.opsem.
 Require Import isla.spec_itree.
+
+Global Hint Transparent sail_name accessor_list : itree_auto.
+
+
+  Lemma bvn_to_bv_to_bvn n (b : bv n) :
+    bvn_to_bv n b = Some b.
+  Proof.
+    rewrite /bvn_to_bv. case_decide as Heq => //. destruct (bv_to_bvn b) eqn:Heq2.
+    by simplify_K.
+  Qed.
+
 
 Global Instance base_val_eq_decision : EqDecision base_val.
 Proof. solve_decision. Qed.
@@ -89,13 +100,25 @@ Definition get_state {S} `{!stateE S -< E} : itree E S :=
 Definition set_state {S} `{!stateE S -< E} (s : S) : itree E unit :=
   trigger (ESetState s).
 
+Lemma get_state_to_translate {E1 E2 S} (HE1 : stateE S -< E1) (HE2 : stateE S -< E2) (Hin : E1 -< E2) :
+  TranslateReSum Hin HE1 HE2 →
+  ITreeToTranslate get_state Hin get_state.
+Proof. move => ?. rewrite /get_state. by apply trigger_to_translate. Qed.
+Global Hint Resolve get_state_to_translate : itree_auto.
+Lemma set_state_to_translate {E1 E2 S} s (HE1 : stateE S -< E1) (HE2 : stateE S -< E2) (Hin : E1 -< E2) :
+  TranslateReSum Hin HE1 HE2 →
+  ITreeToTranslate (set_state s) Hin (set_state s).
+Proof. move => ?. rewrite /set_state. by apply trigger_to_translate. Qed.
+Global Hint Resolve set_state_to_translate : itree_auto.
+
+
 Record seq_state := {
    seq_local : seq_local_state;
    seq_global : seq_global_state;
 }.
 Global Instance eta_seq_state : Settable _ := settable! Build_seq_state <seq_local; seq_global>.
 
-Definition islarisE : Type → Type := demonicE +' specE +' stateE seq_state +' haltE +' ubE.
+Definition islaE : Type → Type := demonicE +' specE +' stateE seq_state +' laterE +' haltE +' ubE.
 
 Definition base_val_to_bool (v : base_val) : option bool :=
   match v with
@@ -109,8 +132,172 @@ Definition val_to_bits (n : N) (v : valu) : option (bv n) :=
   | _ => None
   end.
 
+Definition read_reg {E} `{!stateE seq_state -< E} `{!ubE -< E} (r : string) (al : accessor_list) : itree E valu :=
+  s ← get_state;
+  v ← (s.(seq_local).(seq_regs) !! r)?;
+  read_accessor al v?.
+
+Lemma read_reg_to_translate {E1 E2} r al
+  (HE1 : stateE seq_state -< E1) (HE2 : stateE seq_state -< E2)
+  (Hub1 : ubE -< E1) (Hub2 : ubE -< E2) (Hin : E1 -< E2) :
+  TranslateReSum Hin HE1 HE2 →
+  TranslateReSum Hin Hub1 Hub2 →
+  ITreeToTranslate (read_reg r al) Hin (read_reg r al).
+Proof.
+  move => ??. rewrite /read_reg.
+  apply bind_to_translate; [by apply get_state_to_translate|]. move => ?.
+  apply bind_to_translate; [by apply some_or_ub_to_translate|]. move => ?.
+  by apply some_or_ub_to_translate.
+Qed.
+Global Hint Resolve read_reg_to_translate : itree_auto.
+
+
+Definition write_reg {E} `{!stateE seq_state -< E} `{!ubE -< E} (r : string) (al : accessor_list) (v : valu) : itree E unit :=
+  s ← get_state;
+  vold ← (s.(seq_local).(seq_regs) !! r)?;
+  vnew ← (write_accessor al vold v)?;
+  set_state (s <|seq_local; seq_regs := <[r := vnew]> s.(seq_local).(seq_regs) |>).
+
+Lemma write_reg_to_translate {E1 E2} r al v
+  (HE1 : stateE seq_state -< E1) (HE2 : stateE seq_state -< E2)
+  (Hub1 : ubE -< E1) (Hub2 : ubE -< E2) (Hin : E1 -< E2) :
+  TranslateReSum Hin HE1 HE2 →
+  TranslateReSum Hin Hub1 Hub2 →
+  ITreeToTranslate (write_reg r al v) Hin (write_reg r al v).
+Proof.
+  move => ??. rewrite /write_reg.
+  apply bind_to_translate; [by apply get_state_to_translate|]. move => ?.
+  apply bind_to_translate; [by apply some_or_ub_to_translate|]. move => ?.
+  apply bind_to_translate; [by apply some_or_ub_to_translate|]. move => ?.
+  by apply set_state_to_translate.
+Qed.
+Global Hint Resolve write_reg_to_translate : itree_auto.
+
+Definition read_mem_checked {E} `{!stateE seq_state -< E} `{!ubE -< E} (addr : bv 64) (len : N) : itree E (option bvn) :=
+  s ← get_state;
+  assert (0 < Z.of_N len);;
+  if read_mem s.(seq_global).(seq_mem) (bv_unsigned addr) len is Some m then
+    Ret (Some m)
+  else
+    assert (bv_unsigned addr + Z.of_N len ≤ 2 ^ 64);;
+    assert (set_Forall (λ a, ¬ (bv_unsigned addr ≤ bv_unsigned a < bv_unsigned addr + Z.of_N len)) (dom s.(seq_global).(seq_mem)));;
+    Ret None.
+
+Lemma read_mem_checked_to_translate {E1 E2} addr len
+  (HE1 : stateE seq_state -< E1) (HE2 : stateE seq_state -< E2)
+  (Hub1 : ubE -< E1) (Hub2 : ubE -< E2) (Hin : E1 -< E2) :
+  TranslateReSum Hin HE1 HE2 →
+  TranslateReSum Hin Hub1 Hub2 →
+  ITreeToTranslate (read_mem_checked addr len) Hin (read_mem_checked addr len).
+Proof.
+  move => ??. rewrite /read_mem_checked.
+  apply bind_to_translate; [by apply get_state_to_translate|]. move => ?.
+  apply bind_to_translate; [by apply assert_to_translate|]. move => ?.
+  case_match.
+  - by apply Ret_to_translate.
+  - apply bind_to_translate; [by apply assert_to_translate|]. move => ?.
+    apply bind_to_translate; [by apply assert_to_translate|]. move => ?.
+    by apply Ret_to_translate.
+Qed.
+Global Hint Resolve read_mem_checked_to_translate : itree_auto.
+
+
 Definition compile_trace' (t : isla_trace) :
-  itree (callE isla_trace void +' islarisE) void :=
+  itree (callE isla_trace void +' islaE) void :=
+  later.step;;
+  match t with
+  | Smt (DeclareConst x ty) ann :t: es =>
+      v ← (match ty with
+           | Ty_BitVec b =>
+               n ← demonic Z;
+               Hwf ← assume (BvWf b n);
+               Ret (Val_Bits (@BV b n Hwf))
+           | Ty_Bool =>
+               b ← demonic bool;
+               Ret (Val_Bool b)
+           | Ty_Enum i =>
+               c ← demonic _;
+               Ret (Val_Enum c)
+           | _ => ub
+           end);
+      call (subst_trace v x es)
+  | Smt (DefineConst x e) ann :t: es =>
+      v ← eval_exp e?;
+      call (subst_trace v x es)
+  | Smt (Assert e) ann :t: es =>
+      v ← eval_exp e?;
+      b ← base_val_to_bool v?;
+      assume b;;
+      call es
+  | Assume e ann :t: es =>
+      s ← get_state;
+      v ← eval_a_exp s.(seq_local).(seq_regs) e?;
+      b ← base_val_to_bool v?;
+      assert b;;
+      call es
+  | AssumeReg r al v ann :t: es =>
+      v' ← read_reg r al;
+      assert (v' = v);;
+      call es
+  | ReadReg r al v ann :t: es =>
+      v' ← read_reg r al;
+      vread ← (read_accessor al v)?;
+      assume (vread = v');;
+      call es
+  | WriteReg r al v ann :t: es =>
+      vnew ← (read_accessor al v)?;
+      write_reg r al vnew;;
+      call es
+  | ReadMem data kind addr len tag ann :t: es =>
+      addr' ← (val_to_bits 64 addr)?;
+      data' ← (val_to_bits (8 * len) data)?;
+      res ← read_mem_checked addr' len;
+      if res is Some databvn then
+        data'' ← (bvn_to_bv (8 * len) databvn)?;
+        assume (data' = data'');;
+        call es
+      else
+        emit_label (SReadMem addr' data');;
+        call es
+  | WriteMem res kind addr data len tag ann :t: es =>
+      addr' ← (val_to_bits 64 addr)?;
+      data' ← (val_to_bits (8 * len) data)?;
+      res ← read_mem_checked addr' len;
+      if res is Some _ then
+        s ← get_state;
+        let mem' := write_mem len s.(seq_global).(seq_mem) addr' (bv_unsigned data') in
+        set_state (s <|seq_global;seq_mem := mem'|>);;
+        call es
+      else
+        emit_label (SWriteMem addr' data');;
+        call es
+  | tcases ts =>
+      assert (ts ≠ []);;
+      es ← demonic _;
+      assume (es ∈ ts);;
+      call es
+  | tnil =>
+      s ← get_state;
+      vpc ← read_reg s.(seq_local).(seq_pc_reg) [];
+      pc ← (val_to_bits 64 vpc)?;
+      match s.(seq_global).(seq_instrs) !! pc with
+      | Some es' => call es'
+      | None => emit_label (SInstrTrap pc);; halt
+      end
+  | BranchAddress v ann :t: es => call es
+  | Branch c desc ann :t: es => call es
+  | Barrier v ann :t: es => call es
+  | AbstractPrimop n v args ann :t: es => call es
+  | _ => ub
+  end.
+Global Arguments compile_trace' !_ /.
+
+Definition compile_trace : isla_trace → itree islaE void := rec compile_trace'.
+Global Arguments compile_trace !_ /.
+
+Definition compile_trace_direct_translation' (t : isla_trace) :
+  itree (callE isla_trace void +' islaE) void :=
+  later.step;;
   match t with
   | Smt (DeclareConst x (Ty_BitVec b)) ann :t: es =>
       n ← demonic Z;
@@ -203,5 +390,3 @@ Definition compile_trace' (t : isla_trace) :
   | AbstractPrimop n v args ann :t: es => call es
   | _ => ub
   end.
-
-Definition compile_trace : isla_trace → itree islarisE void := rec compile_trace'.
